Makefile
@@ -4,9 +4,10 @@ all:
 	coqc Memory.v
 	coqc Value.v
 	coqc Lang.v
+	coqc LoadStore.v
 	coqc State.v
 	coqc Behaviors.v
-	coqc LoadStore.v WellTyped.v
+	coqc WellTyped.v
 	coqc SmallStep.v
 	coqc Refinement.v
 	coqc Reordering.v
